tests/lean/run/grind_ematch2.lean
@@ -40,6 +40,47 @@ example (as bs cs : Array α) (v₁ v₂ : α)
         : cs[j] = as[j] := by
   grind
 
+/--
+info: [grind] Counters
+  [thm] E-Matching instances
+    [thm] Array.get_set_ne ↦ 3
+    [thm] Array.size_set ↦ 3
+  [cases] Case splits
+    [cases] And ↦ 2
+---
+info: [diag] Diagnostics
+  [reduction] unfolded declarations (max: 11822, num: 2):
+    [reduction] LT.lt ↦ 11822
+    [reduction] getElem ↦ 64
+  [reduction] unfolded instances (max: 32, num: 1):
+    [reduction] Array.instGetElemNatLtSize ↦ 32
+  [reduction] unfolded reducible declarations (max: 7079, num: 7):
+    [reduction] Array.size ↦ 7079
+    [reduction] Array.toList ↦ 1885
+    [reduction] autoParam ↦ 1694
+    [reduction] outParam ↦ 124
+    [reduction] Ne ↦ 57
+    [reduction] GT.gt ↦ 40
+    [reduction] List.casesOn ↦ 24
+  [def_eq] heuristic for solving `f a =?= f b` (max: 5067, num: 2):
+    [def_eq] Nat.lt ↦ 5067
+    [def_eq] List.length ↦ 1691
+  [kernel] unfolded declarations (max: 106, num: 5):
+    [kernel] LT.lt ↦ 106
+    [kernel] outParam ↦ 46
+    [kernel] Array.size ↦ 36
+    [kernel] Array.toList ↦ 31
+    [kernel] autoParam ↦ 26
+  use `set_option diagnostics.threshold <num>` to control threshold for reporting counters
+---
+info: [grind.ematch.instance] Array.size_set: (cs.set i₃ v₃ ⋯).size = cs.size
+[grind.ematch.instance] Array.size_set: (bs.set i₂ v₂ ⋯).size = bs.size
+[grind.ematch.instance] Array.size_set: (as.set i₁ v₁ ⋯).size = as.size
+[grind.ematch.instance] Array.get_set_ne: ∀ (hj : j < cs.size), i₃ ≠ j → (cs.set i₃ v₃ ⋯)[j] = cs[j]
+[grind.ematch.instance] Array.get_set_ne: ∀ (hj : j < bs.size), i₂ ≠ j → (bs.set i₂ v₂ ⋯)[j] = bs[j]
+[grind.ematch.instance] Array.get_set_ne: ∀ (hj : j < as.size), i₁ ≠ j → (as.set i₁ v₁ ⋯)[j] = as[j]
+-/
+#guard_msgs (info) in
 example (as bs cs ds : Array α) (v₁ v₂ v₃ : α)
         (i₁ i₂ i₃ j : Nat)
         (h₁ : i₁ < as.size)
@@ -52,6 +93,7 @@ example (as bs cs ds : Array α) (v₁ v₂ v₃ : α)
         (h₇ : j < ds.size)
         (h₈ : j < as.size)
         : ds[j] = as[j] := by
+  set_option diagnostics true in
   grind
 
 opaque f (a b : α) : α := a
